examples/acl2/ml/polytypicLib.sml
@@ -618,7 +618,7 @@ let	val (xvar,body) = dest_forall term handle e => wrapException "CASE_SPLIT_CON
 		handle e => raise (mkStandardExn "CASE_SPLIT_CONV"
 				("An nchotomy does not exist for the type of the " ^
 				 " universally quantified variable: " ^ type_to_string t))
-	val nchot = SPEC xvar nchot_thm
+	val nchot = ISPEC xvar nchot_thm
 		handle e => raise (mkDebugExn "CASE_SPLIT_CONV"
 			("TypeBase returned an nchotomy for type " ^ type_to_string t ^
 			 " which was not universally quantified with a variable of the same type!"))
